and more refactorings

theories/Checkers/Functions.v
@@ -1,4 +1,4 @@
-(** * LogRel.Decidability.Functions: conversion and type-checker implementation. *)
+(** * LogRel.Checkers.Functions: conversion and type-checker implementation. *)
 From Coq Require Import Nat Lia.
 From Equations Require Import Equations.
 From PartialFun Require Import Monad PartialFun MonadExn.
@@ -73,6 +73,21 @@ Instance callablePropsDuo {F1 F2} (f1 : F1) (f2 : F2) `{PFun F1 f1, PFun F2 f2} 
 
 Definition call_single {F}
   (f : F) `{PFun F f} {A B} := ext_call (mkSing f) (A:=A) (B:=B).
+
+
+(* The combinator rec throws in a return branch with a type 
+  necessarily convertible to the exception errors type, but the syntactic 
+  mismatch between the 2 types prevents `rec_graph` from `apply`ing.
+  This tactic fixes the type in the return branch to what's expected
+  syntactically. *)
+  Ltac patch_rec_ret :=
+    try (unfold rec;
+    match goal with 
+    | |- orec_graph _ (_rec _ (fun _ : ?Bx => _)) ?hBa => 
+      let Ba := type of hBa in change Bx with Ba
+    end).
+
+
 
 
 #[global]
@@ -174,6 +189,9 @@ Section Views.
     | nf_view1_id _ _ => ty_view1_anomaly
     end.
 
+    (** Comparison of two types in weak-head normal forms, which either have the same
+      head constructor or are mismatched. *)
+
     Inductive nf_ty_view2 : term -> term -> Type :=
     | ty_sorts (s1 s2 : sort) : nf_ty_view2 (tSort s1) (tSort s2)
     | ty_prods (A A' B B' : term) :
@@ -214,6 +232,12 @@ Section Views.
       | ty_view1_anomaly,_ := ty_anomaly _ _ ;
       | _, ty_view1_anomaly := ty_anomaly _ _;
     }.
+
+  (** Comparison of a type and two terms in weak-head normal form, for typed conversion.
+  We have three possibilities:
+  - the type is negative
+  - the type is positive, and the terms have the same head constructor (or are both neutral)
+  - the type is positive, and the terms are mismatched *)
 
   Inductive nf_view3 : term -> term -> term -> Type :=
   | types {A A'} (s : sort) : nf_ty_view2 A A' -> nf_view3 (tSort s) A A'
@@ -278,6 +302,9 @@ Section Views.
     | ty_view1_anomaly := anomaly _ _ _ ;
     }.
 
+
+  (** Comparison of two neutrals in weak-head normal form, for neutral comparison. *)
+
   Inductive ne_view2 : term -> term -> Type :=
     | ne_rels (n n' : nat) : ne_view2 (tRel n) (tRel n')
     | ne_apps f u f' u' : ne_view2 (tApp f u) (tApp f' u')
@@ -308,6 +335,96 @@ Section Views.
       }
       | _, _ := ne_anomaly _ _
     }.
+
+  (** Comparison of two terms in weak-head normal form, for untyped conversion. *)
+
+  Inductive nf_view2 : term -> term -> Type :=
+    | sorts2 (s1 s2 : sort) : nf_view2 (tSort s1) (tSort s2)
+    | prods2 (A A' B B' : term) :
+        nf_view2 (tProd A B) (tProd A' B')
+    | nats2 : nf_view2 tNat tNat
+    | emptys2 : nf_view2 tEmpty tEmpty
+    | sigs2 (A A' B B' : term) : nf_view2 (tSig A B) (tSig A' B')
+    | ids2 A A' x x' y y' : nf_view2 (tId A x y) (tId A' x' y')
+    | lams2 A A' t t' : nf_view2 (tLambda A t) (tLambda A' t')
+    | lam_ne2 A t n' : nf_view2 (tLambda A t) n'
+    | ne_lam2 n A' t' : nf_view2 n (tLambda A' t')
+    | zeros2 : nf_view2 tZero tZero
+    | succs2 t t' : nf_view2 (tSucc t) (tSucc t')
+    | pairs2 A A' B B' t t' u u' :
+        nf_view2 (tPair A B t u) (tPair A' B' t' u')
+    | pair_ne2 A B t u n' :
+        nf_view2 (tPair A B t u) n'
+    | ne_pair2 n A' B' t' u' :
+        nf_view2 n (tPair A' B' t' u')
+    | refls2 A A' x x' : nf_view2 (tRefl A x) (tRefl A' x')
+    | neutrals2 (n n' : term) : nf_view2 n n'
+    | mismatch2 (t u : term) : nf_view2 t u
+    | anomaly2 (t u : term) : nf_view2 t u.
+    
+  Equations build_nf_view2 (t t' : term) : nf_view2 t t' :=
+    build_nf_view2 t t' with (build_nf_view1 t) := {
+    | nf_view1_type (eSort s) with (build_nf_view1 t') := {
+      | nf_view1_type (eSort s') := sorts2 s s' ;
+      | nf_view1_type _ := mismatch2 _ _ ;
+      | nf_view1_ne _ := mismatch2 _ _ ;
+      | _ := anomaly2 _ _ } ;
+    | nf_view1_type (eProd A B) with (build_nf_view1 t') := {
+      | nf_view1_type (eProd A' B') := prods2 A A' B B' ;
+      | nf_view1_type _ := mismatch2 _ _ ;
+      | nf_view1_ne _ := mismatch2 _ _ ;
+      | _ := anomaly2 _ _ } ;
+    | nf_view1_type eNat with (build_nf_view1 t') := {
+      | nf_view1_type eNat := nats2 ;
+      | nf_view1_type _ := mismatch2 _ _ ;
+      | nf_view1_ne _ := mismatch2 _ _ ;
+      | _ := anomaly2 _ _ } ;
+    | nf_view1_type eEmpty with (build_nf_view1 t') := {
+      | nf_view1_type eEmpty := emptys2 ;
+      | nf_view1_type _ := mismatch2 _ _ ;
+      | nf_view1_ne _ := mismatch2 _ _ ; 
+      | _ := anomaly2 _ _ } ;
+    | nf_view1_type (eSig A B) with (build_nf_view1 t') := {
+      | nf_view1_type (eSig A' B') := sigs2 A A' B B' ;
+      | nf_view1_type _ := mismatch2 _ _ ;
+      | nf_view1_ne _ := mismatch2 _ _ ;
+      | _ := anomaly2 _ _ } ;
+    | nf_view1_type (eId A x y) with (build_nf_view1 t') := {
+      | nf_view1_type (eId A' x' y') := ids2 A A' x x' y y' ;
+      | nf_view1_type _ := mismatch2 _ _ ;
+      | nf_view1_ne _ := mismatch2 _ _ ;
+      | _ := anomaly2 _ _ } ;
+    | nf_view1_fun A t with (build_nf_view1 t') := {
+      | nf_view1_fun A' t' := lams2 A A' t t' ;
+      | nf_view1_ne _ := lam_ne2 A t _ ; 
+      | _ := anomaly2 _ _ } ;
+    | nf_view1_nat eZero with (build_nf_view1 t') := {
+      | nf_view1_nat eZero := zeros2 ;
+      | nf_view1_nat (eSucc _) := mismatch2 _ _ ;
+      | nf_view1_ne _ := mismatch2 _ _ ; 
+      | _ := anomaly2 _ _ } ;
+    | nf_view1_nat (eSucc u) with (build_nf_view1 t') := {
+      | nf_view1_nat (eSucc u') := succs2 u u' ;
+      | nf_view1_nat eZero := mismatch2 _ _ ;
+      | nf_view1_ne _ := mismatch2 _ _ ; 
+      | _ := anomaly2 _ _ } ;
+    | nf_view1_sig A B t u with (build_nf_view1 t') := {
+      | nf_view1_sig A' B' t' u' := pairs2 A A' B B' t t' u u' ;
+      | nf_view1_ne _ := pair_ne2 A B t u _ ; 
+      | _ := anomaly2 _ _ } ;
+    | nf_view1_id A x with (build_nf_view1 t') := {
+      | nf_view1_id A' x' := refls2 A A' x x' ;
+      | nf_view1_ne _ := mismatch2 _ _ ;
+      | _ := anomaly2 _ _ } ;
+    | nf_view1_ne _ with (build_nf_view1 t') := {
+      | nf_view1_type _ := mismatch2 _ _ ;
+      | nf_view1_fun A' t' := ne_lam2 _ A' t' ;
+      | nf_view1_nat _ := mismatch2 _ _ ;
+      | nf_view1_sig A' B' t' u' := ne_pair2 _ A' B' t' u' ;
+      | nf_view1_id _ _ := mismatch2 _ _ ;
+      | nf_view1_ne _ := neutrals2 _ _ ;
+    }
+  }.
 
 End Views.
 
@@ -571,6 +688,120 @@ Equations tconv : (context × term × term) ⇀ exn errors unit :=
 End Conversion.
 
 #[export] Instance: PFun tconv := pfun_gen _ _ tconv.
+
+
+(** ** Untyped conversion *)
+
+Section Conversion.
+
+Definition uconv_dom := conv_state × term × term.
+Definition uconv_cod (_ : uconv_dom) := exn errors unit.
+
+#[local]
+Notation M0 := (orec (Sing wh_red) (uconv_dom) (uconv_cod)).
+#[local]
+Notation M := (combined_orec (exn errors) (Sing wh_red) uconv_dom uconv_cod).
+
+Equations uconv_tm : (term × term) -> M unit :=
+  | (t,u) :=
+    t' ← call_single wh_red t ;;[M0]
+    u' ← call_single wh_red u ;;[M0]
+    rec (tm_red_state,t',u').
+    
+Equations uconv_tm_red : (term × term) -> M unit :=
+  | (t,t') with (build_nf_view2 t t') :=
+  {
+    | sorts2 s s' :=
+        ret (eq_sort s s') ;
+    | prods2 A A' B B' :=
+        rec (tm_state,A,A') ;;
+        rec (tm_state,B,B') ;
+    | nats2 := ok ;
+    | emptys2 := ok ;
+    | sigs2 A A' B B' :=
+        rec (tm_state,A,A') ;;
+        rec (tm_state,B,B') ;
+    | ids2 A A' x x' y y' :=
+        rec (tm_state,A,A') ;;
+        rec (tm_state,x,x') ;;
+        rec (tm_state,y,y') ;
+    | lams2 _ _ t t' :=
+        rec (tm_state,t,t') ;
+    | lam_ne2 _ t t' :=
+        rec (tm_state,t,eta_expand t') ;
+    | ne_lam2 t _ t' :=
+        rec (tm_state,eta_expand t,t') ;
+    | zeros2 := ok ;
+    | succs2 t t' :=
+        rec (tm_state,t,t') ;
+    | pairs2 _ _ _ _ t t' u u' :=
+        rec (tm_state,t,t') ;;
+        rec (tm_state,u,u') ;
+    | pair_ne2 _ _ t u t' :=
+        rec (tm_state,t,tFst t') ;;
+        rec (tm_state,u,tSnd t') ;
+    | ne_pair2 t _ _ t' u' :=
+        rec (tm_state,tFst t, t') ;;
+        rec (tm_state,tSnd t,u') ;
+    | refls2 A A' x x' := 
+      ok ;
+    | neutrals2 _ _ :=
+      rec (ne_state,t,t') ;
+    | mismatch2 _ _ := raise head_mismatch ;
+    | anomaly2 _ _ := undefined ;
+  }.
+
+Equations uconv_ne : (term × term) -> M unit :=
+  uconv_ne (t,t') with build_ne_view2 t t' :=
+  {
+  | ne_rels n n' with n =? n' :=
+    { | false := raise variable_mismatch ;
+      | true := ok ;
+    } ;
+      
+  | ne_apps n t n' t' :=
+    rec (ne_state,n,n') ;;
+    rec (tm_state,t,t') ;
+
+  | ne_nats n P hz hs n' P' hz' hs' :=
+    rec (ne_state,n,n') ;;
+    rec (tm_state,P,P') ;;
+    rec (tm_state,hz,hz') ;;
+    rec (tm_state,hs,hs')
+
+  | ne_emptys n P n' P' :=
+    rec (ne_state,n,n') ;;
+    rec (tm_state,P,P')
+
+  | ne_fsts n n' :=
+    rec (ne_state,n,n')
+
+  | ne_snds n n' :=
+    rec (ne_state,n,n')
+
+  | ne_ids A x P hr y n A' x' P' hr' y' n' :=
+      rec (ne_state,n,n') ;;
+      rec (tm_state,P,P') ;;
+      rec (tm_state,hr,hr') ;
+
+  | ne_mismatch _ _ => raise destructor_mismatch ;
+  | ne_anomaly _ _ => undefined
+}.
+
+Equations _uconv : ∇ _ : conv_state × term × term, [Sing wh_red]⇒[exn errors] unit :=
+  | (tm_state,t,u) := uconv_tm (t,u) ;
+  | (tm_red_state,t,u) := uconv_tm_red (t,u);
+  | (ne_state,t,u) := uconv_ne (t,u) ;
+  | (_,t,u) := undefined.
+
+  #[local] Instance: PFun _uconv := pfun_gen _ _ _uconv.
+
+  Equations uconv : (context × term × term) ⇀ exn errors unit :=
+    uconv (Γ,T,V) := call _uconv (tm_state,T,V).
+  
+End Conversion.
+
+#[export] Instance: PFun uconv := pfun_gen _ _ uconv.
 
 
 (** ** Typing *)
