theories/Checkers/CtxAccessCorrectness.v
@@ -1,0 +1,49 @@
+(** * LogRel.Checkers.CtxAccessCorrectness: correctness of the context accessing function. *)
+From Coq Require Import Nat Lia Arith.
+From Equations Require Import Equations.
+From LogRel Require Import Utils Syntax.All.
+
+From LogRel.Checkers Require Import Functions.
+From PartialFun Require Import Monad PartialFun MonadExn.
+
+Set Universe Polymorphism.
+
+(** ** Correctness of context access *)
+(** The function is equivalent to the in_ctx predicate. *)
+
+Section CtxAccessCorrect.
+
+  Lemma ctx_access_sound Γ n d :
+    ctx_access Γ n = success d ->
+    in_ctx Γ n d.
+  Proof.
+    funelim (ctx_access Γ n).
+    all: simp ctx_access ; cbn.
+    - inversion 1.
+    - inversion 1.
+      now constructor.
+    - destruct (ctx_access Γ n') ; cbn.
+      all: inversion 1 ; subst.
+      constructor.
+      now apply H.
+  Qed.
+
+  Lemma ctx_access_complete Γ n d :
+    in_ctx Γ n d ->
+    ctx_access Γ n = success d.
+  Proof.
+    induction 1.
+    all: simp ctx_access ; cbn.
+    - reflexivity.
+    - now rewrite IHin_ctx. 
+  Qed.
+
+  Corollary ctx_access_correct Γ n d :
+    in_ctx Γ n d <~> (ctx_access Γ n = success d).
+  Proof.
+    split.
+    - eapply ctx_access_complete.
+    - eapply ctx_access_sound.
+  Qed.
+
+End CtxAccessCorrect.
