theories/Checkers/ReductionCorrectness.v
@@ -1,0 +1,374 @@
+(** * LogRel.Checkers.ReductionCorrectness: properties of the reduction function. *)
+From Coq Require Import Nat Lia Arith.
+From Equations Require Import Equations.
+From LogRel Require Import Syntax.All DeclarativeTyping GenericTyping AlgorithmicJudgments.
+From LogRel.TypingProperties Require Import NormalisationDefinition DeclarativeProperties PropertiesDefinition SubstConsequences TypeInjectivityConsequences NeutralConvProperties.
+From LogRel.Algorithmic Require Import Bundled TypedConvProperties AlgorithmicTypingProperties.
+From LogRel Require Import Utils.
+
+From LogRel.Checkers Require Import Functions Views.
+From PartialFun Require Import Monad PartialFun MonadExn.
+
+Set Universe Polymorphism.
+#[global] Unset Asymmetric Patterns.
+
+Import DeclarativeTypingProperties.
+
+
+Lemma zip_ored t t' π : [t ⤳ t'] -> [zip t π ⤳ zip t' π].
+Proof.
+  intros Hred.
+  induction π as [|[]] in t, t', Hred |- * ; cbn in *.
+  1: eassumption.
+  all: apply IHπ ; now econstructor.
+Qed.
+
+Lemma zip_red t t' π : [t ⤳* t'] -> [zip t π ⤳* zip t' π].
+Proof.
+  induction 1.
+  1: reflexivity.
+  econstructor ; tea.
+  now eapply zip_ored.
+Qed.
+
+(** ** Soundness of reduction *)
+(** If the reduction function called on a term t returns a term t', then
+t reduces to t' and t' is a weak-head normal form. *)
+
+Section RedImplemSound.
+
+Lemma red_stack_sound :
+  funrec wh_red_stack (fun _ => True) (fun '(t,π) t' => [zip t π ⤳* t']).
+Proof.
+  intros ? _.
+  funelim (wh_red_stack _).
+  all: cbn ; econstructor ; try eauto.
+  all: intros v ?.
+  all: etransitivity ; [..|eassumption].
+  all: eapply zip_red.
+  all: econstructor ; [..|reflexivity].
+  all: now econstructor.
+Qed.
+
+Lemma stack_ne n π :
+  whne n -> whne (zip n π).
+Proof.
+  intros Hne.
+  induction π as [|[]] in n, Hne |- * ; cbn.
+  1: eassumption.
+  all: eapply IHπ ; now econstructor.
+Qed.
+
+Lemma red_stack_whnf :
+funrec wh_red_stack (fun _ => True) (fun '(t,π) t' => whnf t').
+Proof.
+  intros ? _.
+  funelim (wh_red_stack _).
+  all: cbn ; try solve [constructor ; eauto]. 
+  - now eapply isType_whnf, isType_tm_view1.
+  - econstructor. eapply stack_ne.
+    now econstructor.
+  - now eapply whnf_tm_view1_nat.
+Qed.
+
+Corollary _red_sound :
+  funrec wh_red (fun _ => True) (fun t t' => [t ⤳* t'] × whnf t').
+Proof.
+  intros ? _.
+  cbn; intros ? H; split.
+  - eapply funrec_graph in H.
+    2: apply red_stack_sound.
+    all: easy.
+  - eapply funrec_graph in H.
+    2: exact red_stack_whnf.
+    all: easy.
+Qed.
+
+#[universes(polymorphic)]Corollary red_sound t t' :
+  graph wh_red t t' ->
+  [t ⤳* t'] × whnf t'.
+Proof.
+  intros H.
+  pattern t, t'.
+  eapply funrec_graph.
+  1: apply _red_sound.
+  all: easy.
+Qed.
+
+End RedImplemSound.
+
+(** ** Completeness of reduction *)
+(** Given any well-formed input, which reduces to a weak-head normal form, the reduction function finds
+  that weak-head normal form. This does not rely on normalisation, since we assume a reduction relation. *)
+
+Section RedImplemComplete.
+  Context `{!TypingSubst de} `{!TypeConstructorsInj de}.
+
+  #[local]Definition R_aux := lexprod term term cored term_subterm.
+
+  #[local]Definition R (t u : term × stack) :=
+    R_aux (Datatypes.pair (zip (fst t) (snd t)) (fst t)) (Datatypes.pair (zip (fst u) (snd u)) (fst u)).
+
+  Lemma R_acc t π :
+    Acc cored (zip t π) ->
+    Acc R (t, π).
+  Proof.
+  intros h.
+  eapply acc_A_B_lexprod with (leA := cored) (leB := term_subterm) (y := t) in h.
+  - remember (Datatypes.pair (zip t π) t) as z eqn:e.
+    induction h as [z h ih] in t, π, e |- *. subst.
+    constructor. intros [v ρ] hr.
+    unfold R, R_aux in hr ; cbn in *.
+    eapply ih. 2: reflexivity.
+    assumption.
+  - eapply well_founded_term_subterm.
+  - eapply well_founded_term_subterm.
+  Qed.
+
+  Lemma normalising_acc t π t' :
+    [(zip t π) ⤳* t'] ->
+    whnf t' ->
+    Acc R (t,π).
+  Proof.
+    intros Hred Hnf.
+    eapply R_acc.
+    set (t'' := (zip t π)) in *.
+    clearbody t''.
+    clear -Hred Hnf.
+    induction Hred.
+    - constructor.
+      intros ? [].
+      now edestruct whnf_nored.
+    - constructor.
+      now eintros ? [<-%ored_det].
+  Qed.
+
+  Lemma well_typed_zip Γ t π :
+    well_typed (ta := de) Γ (zip t π) ->
+    ∑ T', [Γ |-[de] t : T'] × (forall u, [Γ |-[de] t ≅ u : T'] -> well_typed (ta := de) Γ (zip u π)).
+  Proof.
+    intros H.
+    induction π as [|[]] in t, H |- * ; cbn.
+    - destruct H as [T Hty].
+      exists T ; split.
+      1: eassumption.
+      intros *.
+      eexists.
+      boundary.
+    - cbn in H.
+      eapply IHπ in H as (T&(?&[]&?)%termGen'&Hsubst) ; subst.
+      eexists ; split ; tea.
+      intros u Htyu.
+      eapply Hsubst.
+      econstructor.
+      1: eapply TermEmptyElimCong ; tea ; refold.
+      2: eassumption.
+      now econstructor.
+    - cbn in H.
+      eapply IHπ in H as (T&(?&[]&?)%termGen'&Hsubst) ; subst.
+      eexists ; split ; tea.
+      intros u Htyu.
+      eapply Hsubst.
+      econstructor.
+      1: eapply TermNatElimCong ; tea ; refold.
+      + now econstructor.
+      + now econstructor.
+      + now eapply TermRefl.
+      + eassumption.
+    - cbn in H.
+      eapply IHπ in H as (T&(?&(?&?&[])&?)%termGen'&Hsubst) ; subst.
+      eexists ; split ; tea.
+      intros u' Htyu.
+      eapply Hsubst.
+      econstructor.
+      1: econstructor ; tea.
+      2: eassumption.
+      now econstructor.
+    - cbn in H.
+      eapply IHπ in H as [T [[?[[?[?[->]]]]]%termGen' Hsubst]].
+      eexists; split; tea.
+      intros; eapply Hsubst.
+      eapply TermConv; refold; tea.
+      now econstructor.
+    - cbn in H.
+      eapply IHπ in H as [T [[?[[?[?[->]]]]]%termGen' Hsubst]].
+      eexists; split; tea.
+      intros; eapply Hsubst.
+      eapply TermConv; refold; tea.
+      now econstructor.
+  - cbn in H.
+    eapply IHπ in H as [T [[? [[->]]]%termGen' Hsubst]].
+      eexists; split; tea.
+      intros; eapply Hsubst.
+      eapply TermConv; refold; tea.
+      econstructor; tea; eapply TypeRefl + eapply TermRefl; refold; tea.
+  Qed.
+
+  Lemma zip1_notType Γ T t π :
+    isType t ->
+    ~ whne t ->
+    ~ [Γ |-[de] zip1 t π : T].
+  Proof.
+    intros Ht Ht' Hty.
+    destruct π ; cbn in * ;
+      eapply termGen' in Hty as (?&[]&?) ; subst ; prod_hyp_splitter ;
+      match goal with H : [_ |-[de] t : _] |- _ => (unshelve eapply isType_ty, ty_conv_inj in H) end ; tea.
+    all: try solve
+      [now econstructor| now eapply not_whne_can ; tea ; eapply isType_whnf | now cbn in *].
+  Qed.
+
+  Ltac termInvContradiction Hty := 
+    eapply termGen' in Hty; cbn in Hty; prod_hyp_splitter; subst;
+    now match goal with 
+    | [H : [_ |-[de] _ : _] |- _] =>
+      eapply termGen' in H; cbn in H; prod_hyp_splitter; subst;
+      now match goal with
+      | [H : [_ |-[de] _ ≅ _] |- _] => unshelve eapply ty_conv_inj in H; first [constructor | easy]
+      end
+    end.
+
+  Lemma wh_red_stack_complete Γ t π t' :
+    well_typed Γ (zip t π) ->
+    [(zip t π) ⤳* t'] ->
+    whnf t' ->
+    domain wh_red_stack (t,π).
+  Proof.
+    intros Hty Hred Hnf.
+    pose proof (Hacc := normalising_acc _ _ _ Hred Hnf).
+    change (zip t π) with (zip (fst (t,π)) (snd (t,π))) in *.
+    set (z := (t, π)) in *. clearbody z.
+    clear Hnf Hred.
+    induction Hacc as [z H IH] in Hty |- *.
+    apply compute_domain. funelim (wh_red_stack z).
+    all: simpl.
+    all: try easy.
+    all: try solve [ cbn in * ; eapply well_typed_zip in Hty as [? [Hty _]] ; cbn in *; termInvContradiction Hty].
+    - cbn in * ; eapply well_typed_zip in Hty as [? [? _]] ; cbn in *.
+      eapply zip1_notType ; tea.
+      all: now eapply isType_tm_view1.
+    - split ; [|easy].
+      eapply IH.
+      + red. red. cbn.
+        left.
+        constructor.
+        eapply zip_ored.
+        now econstructor.
+      + cbn in *.
+        eapply well_typed_zip in Hty as (?&[??Hu]).
+        eapply Hu, RedConvTeC, subject_reduction ; tea.
+        now do 2 econstructor.
+  - split ; [|easy].
+    eapply IH.
+    + red. red. cbn.
+      left.
+      constructor.
+      eapply zip_ored.
+      now econstructor.
+    + cbn in *.
+      eapply well_typed_zip in Hty as (?&[??Hu]).
+      eapply Hu, RedConvTeC, subject_reduction ; tea.
+      now do 2 econstructor.
+  - cbn in *.
+    split ; [|easy].
+    eapply IH ; cbn in *.
+    + red. red. cbn.
+      left.
+      constructor.
+      eapply zip_ored.
+      now econstructor.
+    + cbn in *.
+      eapply well_typed_zip in Hty as (?&[??Hu]).
+      eapply Hu, RedConvTeC, subject_reduction ; tea.
+      now do 2 econstructor.
+  - cbn in *; split; [|easy].
+    eapply IH.
+    + do 2 red; cbn.
+      left; constructor; eapply zip_ored; constructor.
+    + cbn. 
+      eapply well_typed_zip in Hty as (?&[??Hu]).
+      eapply Hu, RedConvTeC, subject_reduction ; tea.
+      now do 2 econstructor.
+  - cbn in *; split; [|easy].
+    eapply IH.
+    + do 2 red; cbn.
+      left; constructor; eapply zip_ored; constructor.
+    + cbn. 
+      eapply well_typed_zip in Hty as (?&[??Hu]).
+      eapply Hu, RedConvTeC, subject_reduction ; tea.
+      now do 2 econstructor.
+  - cbn in *; split;[|easy].
+    eapply IH.
+    + do 2 red; cbn.
+      left; constructor; eapply zip_ored; constructor.
+    + cbn.
+      eapply well_typed_zip in Hty as [? [? Hu]] .
+      eapply Hu, RedConvTeC, subject_reduction; tea.
+      eapply redalg_one_step; constructor.
+  - cbn in *.
+    split ; [|easy].
+    eapply IH ; cbn in *.
+    2: eassumption.
+    red. red. cbn.
+    right.
+    econstructor.
+    destruct s ; cbn ; now constructor.
+  Qed.
+
+  Corollary wh_red_complete Γ t :
+    well_formed Γ t ->
+    normalising t ->
+    domain wh_red t.
+  Proof.
+    intros [|w]%well_formed_well_typed [].
+    all: eapply compute_domain; cbn.
+    all: split ; [|easy].
+    - eapply wh_red_stack_complete ; tea.
+    - inversion w ; subst ; clear w; cycle -1.
+      1: eapply wh_red_stack_complete ; tea ; now econstructor.
+      all: econstructor ; cbn ; red.
+      all: simp wh_red_stack ; cbn.
+      all: now econstructor.
+  Qed.
+
+  Corollary wh_red_complete_whnf_class Γ K t t' :
+  [Γ |- t ⤳* t' ∈ K] ->
+  whnf t' ->
+  graph wh_red t t'.
+  Proof.
+    intros [] ? ; refold.
+    assert (domain wh_red t) as h.
+    {
+      eapply (wh_red_complete Γ).
+      2: now econstructor.
+      destruct K as [|A] ; unshelve econstructor ; [left|right|..] ; cbn.
+      2-3: eassumption.
+    }
+    replace t' with (def wh_red t h).
+    1: eapply def_graph_sound.
+    eapply whred_det ; tea.
+    all: now eapply red_sound, def_graph_sound.
+  Qed.
+  
+  Corollary wh_red_complete_whnf_ty Γ A A' :
+  [Γ |-[de] A] ->
+  [A ⤳* A'] ->
+  whnf A' ->
+  graph wh_red A A'.
+  Proof.
+    intros ? Hred ?.
+    eapply subject_reduction_type in Hred ; tea.
+    now eapply wh_red_complete_whnf_class.
+  Qed.
+  
+  Corollary wh_red_complete_whnf_tm Γ A t t' :
+  [Γ |-[de] t : A] ->
+  [t ⤳* t'] ->
+  whnf t' ->
+  graph wh_red t t'.
+  Proof.
+    intros ? Hred ?.
+    eapply subject_reduction in Hred ; tea.
+    now eapply wh_red_complete_whnf_class.
+  Qed.
+
+End RedImplemComplete.
